# Recursion | Codecademy

# Quiz: Recursion in Java

## Questions

Fill in the `.findNodeRecursively()` method, so it returns the correct node when found, or `null` if not found.

### Code

```
public Node findNodeRecursively(String data, Node currentNode) {Â Â Â Â if (currentNode == null) {Â Â Â Â Â Â Â Â return null;Â Â Â Â } else if (currentNode.data == data) {Â Â Â Â Â Â Â Â return currentNode;Â Â Â Â } else {Â Â Â Â Â Â Â Â return this.findNodeRecursively(data, currentNode.getNextNode());Â Â Â Â }}
```

## Answer Choices

Click or drag and drop to fill in the blank

ğŸ‘

You got it!

## Embedded Content

# Recursion | Codecademy

# Quiz: Recursion in Java

## Questions

Fill in the code, so `recursiveSum()` recursively finds the sum of a number and all positive numbers less than it.

### Code

```
public static int recursiveSum (int n) {Â Â if (n == 1) {Â Â Â Â return 1;Â Â } else {Â Â Â Â return recursiveSum(n - 1) +Â n;Â Â }}
```

## Answer Choices

Click or drag and drop to fill in the blank

ğŸ‘

You got it!

## Embedded Content

# Recursion | Codecademy

# Quiz: Recursion in Java

## Questions

Fill in the code, so `recursiveFactorial()` recursively finds the factorial solution to an argument and returns it.

### Code

```
public static int recursiveFactorial(int n) {Â Â Â if (n > 0) {Â Â Â Â return recursiveFactorial(n - 1) *Â n;Â Â } else {Â Â Â Â Â Â Â Â return 1;Â Â Â Â }}
```

## Answer Choices

-   n == 0

Click or drag and drop to fill in the blank

ğŸ‘

You got it!

## Embedded Content

# Recursion | Codecademy

# Quiz: Recursion in Java

## Questions

Fill in the correct conditions for the `.findNodeRecursively()` method.

### Code

```
public Node findNodeRecursively(String data, Node currentNode) {Â Â Â Â if (currentNode == null) {Â Â Â Â Â Â Â Â return null;Â Â Â Â } else if (currentNode.data == data) {Â Â Â Â Â Â Â Â return currentNode;Â Â Â Â } else {Â Â Â Â Â Â Â Â return this.findNodeRecursively(data, currentNode.getNextNode());Â Â Â Â }}
```

## Answer Choices

-   !(currentNode == null)
-   currentNode.next == null
-   currentNode > 0

Click or drag and drop to fill in the blank

ğŸ‘

You got it!

## Embedded Content

# Recursion | Codecademy

# Quiz: Recursion in Java

## Questions

The code displays a recursive solution to finding a node in a linked list. Which of the following is the condition for the recursive case?

### Code

```
public Node findNodeRecursively(String data, Node currentNode) {Â Â Â Â if (currentNode == null) {Â Â Â Â Â Â Â Â return null;Â Â Â Â } else if (currentNode.data == data) {Â Â Â Â Â Â Â Â return currentNode;Â Â Â Â } else {Â Â Â Â Â Â Â Â return this.findNodeRecursively(data, currentNode.getNextNode());Â Â Â Â }}
```

## Answer Choices

-   `currentNode == null`
-   `currentNode.data == data`
-   (Selected)Correct:

    The recursive condition is if `currentNode.data == data` and `currentNode == null` are not `true`

    ğŸ‘

    Nice work! The recursive case executes if the first two conditions are not true.

## Embedded Content

# Recursion | Codecademy

# Quiz: Recursion in Java

## Questions

Which of the following errors often occurs if you do not include a base case in your recursive function?

## Answer Choices

-   (Selected)Correct:

    A stack overflow

    ğŸ‘

    Nice work! If the function does not have a base case, then it may continue to call itself indefinitely.

-   A value error
-   Key error
-   Import error

## Embedded Content

# Recursion | Codecademy

# Quiz: Recursion in Java

## Questions

The function `recursiveFactorial()` uses recursion to find the factorial solution to the argument passed into it. Which of the following is a realistic call stack for the call `recursiveFactorial(3)`?

## Answer Choices

-   1.  `recursiveFactorial(1)` = `1 * recursiveFactorial(0)`
    2.  `recursiveFactorial(2)` = `2 * recursiveFactorial(1)`
    3.  `recursiveFactorial(3)` = `3 * recursiveFactorial(2)`
-   1.  `recursiveFactorial(2)` = `2 * recursiveFactorial(1)`
    2.  `recursiveFactorial(1)` = `1 * recursiveFactorial(0)`
    3.  `recursiveFactorial(3)` = `3 * recursiveFactorial(2)`
-   1.  `recursiveFactorial(3)` = `3 * recursiveFactorial(2)`
-   (Selected)Correct:

    1.  `recursiveFactorial(3)` = `3 * recursiveFactorial(2)`
    2.  `recursiveFactorial(2)` = `2 * recursiveFactorial(1)`
    3.  `recursiveFactorial(1)` = `1 * recursiveFactorial(0)`

    ğŸ‘

    Nice work! The `recursiveFactorial()` function will call itself with inputs of `0`, `1`, `2`, and `3` and multiply the solution by `n+1` values. The top of tâ€¦

    Show more

## Embedded Content
